lemma_activeVertexHasPathToSource

Flow.dfy
@@ -6,6 +6,76 @@ module FlowGraph {
   type Capacity = c: seq<seq<nat>> | |c| == V && forall i :: 0 <= i < |c| ==> |c[i]| == V witness seq(V, _ => seq(V, _ => 0))
   type Flow = f: seq<seq<int>> | |f| == V && forall i :: 0 <= i < |f| ==> |f[i]| == V witness seq(V, _ => seq(V, _ => 0))
 
+  function ResidualCapacity(c: Capacity, f: Flow, v: Node, w: Node): nat
+    requires ValidCapacityConstraint(c, f)
+  {
+    c[v][w] - f[v][w]
+  }
+
+  // Computes the sum of flow into node 'v' on edges from (0, v) up to edge ('maxSource', v)
+  function SumTotalFlowToNode(f: Flow, v: Node, maxSource: nat): int
+    requires maxSource < V
+    decreases maxSource
+  {
+    if maxSource == 0 then
+      f[0][v]
+    else
+      f[maxSource][v] + SumTotalFlowToNode(f, v, maxSource-1)
+  }
+
+  function SumFlowFromSetToNode(f: Flow, S: set<Node>, v: Node, maxSource: nat): int
+    requires maxSource < V
+    decreases maxSource
+  {
+    (if maxSource in S then f[maxSource][v] else 0) +
+    (if maxSource == 0 then 0 else SumFlowFromSetToNode(f, S, v, maxSource - 1))
+  }
+
+  function SumFlowFromNodeToSet(f: Flow, S: set<Node>, v: Node, maxDest: nat): int
+    requires maxDest < V
+    decreases maxDest
+  {
+    (if maxDest in S then f[v][maxDest] else 0) +
+    (if maxDest == 0 then 0 else SumFlowFromNodeToSet(f, S, v, maxDest - 1))
+  }
+
+  function SumFlowFromAllNodesToSet(f: Flow, S: set<Node>, maxSource: nat, maxDest: nat): int
+    requires maxSource < V && maxDest < V
+    decreases maxSource
+  {
+    SumFlowFromNodeToSet(f, S, maxSource, maxDest) +
+    (if maxSource == 0 then 0 else SumFlowFromAllNodesToSet(f, S, maxSource - 1, maxDest))
+  }
+
+  function SumIncomingFlowOfSet(f: Flow, S: set<Node>, maxSource: nat, maxDest: nat): int
+    requires maxSource < V && maxDest < V
+    decreases maxDest
+  {
+    (if maxDest in S then SumTotalFlowToNode(f, maxDest, maxSource) else 0) +
+    (if maxDest == 0 then 0 else SumIncomingFlowOfSet(f, S, maxSource, maxDest - 1))
+  }
+
+  function SumInternalFlowToSet(f: Flow, S: set<Node>, maxSource: nat, maxDest: nat): int
+    requires maxSource < V && maxDest < V decreases maxSource
+  {
+    (if maxSource in S then SumFlowFromNodeToSet(f, S, maxSource, maxDest) else 0) +
+    (if maxSource == 0 then 0 else SumInternalFlowToSet(f, S, maxSource - 1, maxDest))
+  }
+
+  function SumExternalFlowToSet(f: Flow, S: set<Node>, maxSource: nat, maxDest: nat): int
+    requires maxSource < V && maxDest < V
+    decreases maxSource
+  {
+    (if maxSource !in S then SumFlowFromNodeToSet(f, S, maxSource, maxDest) else 0) +
+    (if maxSource == 0 then 0 else SumExternalFlowToSet(f, S, maxSource - 1, maxDest))
+  }
+
+  ghost function NodesReachableFrom(c: Capacity, f: Flow, v: Node): set<Node>
+    requires ValidCapacityConstraint(c, f)
+  {
+    set w: Node | exists p: Path :: IsSimpleResidualPath(c, f, p) && p[0] == v && p[|p|-1] == w
+  }
+
   predicate ValidCapacityConstraint(c: Capacity, f: Flow)
   {
     forall v: Node, w: Node :: (f[v][w] <= c[v][w])
@@ -18,24 +88,7 @@ module FlowGraph {
 
   predicate ValidFlowConservationConstraint(s: Node, t: Node, f: Flow)
   {
-    forall v: Node {:trigger SumFlowInOnEdgesUpToEdgeUV(f, v, V - 1)} | (v != s && v != t) :: (SumFlowInOnEdgesUpToEdgeUV(f, v, V - 1) == 0)
-  }
-
-  // Computes the sum of flow into node 'v' on edges from (0, v) up to edge ('u', v)
-  function SumFlowInOnEdgesUpToEdgeUV(f: Flow, v: Node, u: nat): int
-    requires u < V
-    decreases u
-  {
-    if u == 0 then
-      f[0][v]
-    else
-      f[u][v] + SumFlowInOnEdgesUpToEdgeUV(f, v, u-1)
-  }
-
-  function ResidualCapacity(c: Capacity, f: Flow, v: Node, w: Node): nat
-    requires ValidCapacityConstraint(c, f)
-  {
-    c[v][w] - f[v][w]
+    forall v: Node {:trigger SumTotalFlowToNode(f, v, V - 1)} | (v != s && v != t) :: (SumTotalFlowToNode(f, v, V - 1) == 0)
   }
 
   predicate ValidFlow(s: Node, t: Node, c: Capacity, f: Flow)
@@ -55,11 +108,160 @@ module FlowGraph {
     IsResidualPath(c, f, p) && IsSimplePath(p)
   }
   
-  lemma Lemma_ZeroFlowHasZeroSum(f: Flow, v: Node, u: nat)
+  lemma Lemma_ZeroFlowEqualsZeroSumFlowInOfNode(f: Flow, v: Node, u: nat)
     requires u < V
     requires forall i: Node, j: Node :: f[i][j] == 0
-    ensures SumFlowInOnEdgesUpToEdgeUV(f, v, u) == 0
+    ensures SumTotalFlowToNode(f, v, u) == 0
   {
     // automatically verified by Dafny
+  }
+
+  lemma Lemma_NodeReachableFromReachableSetIsReachable(c: Capacity, f: Flow, v: Node, n: Node, m: Node)
+    requires ValidCapacityConstraint(c, f)
+    requires n in NodesReachableFrom(c, f, v)
+    requires ResidualCapacity(c, f, n, m) > 0
+    ensures m in NodesReachableFrom(c, f, v)
+  {
+    var p :| IsSimpleResidualPath(c, f, p) && p[0] == v && p[|p|-1] == n;
+    if m in p {
+      var k :| 0 <= k < |p| && p[k] == m;
+      assert IsSimpleResidualPath(c, f, p[..k+1]);
+    } else {
+      assert IsSimpleResidualPath(c, f, p + [m]);
+    }
+  }
+
+  lemma Lemma_SumIncomingFlowOfSetEqualsSumFlowFromAllNodesToSet_Base(f: Flow, S: set<Node>, maxDest: nat)
+    requires maxDest < V
+    ensures SumIncomingFlowOfSet(f, S, 0, maxDest) == SumFlowFromNodeToSet(f, S, 0, maxDest)
+    decreases maxDest
+  {
+    if maxDest > 0 { Lemma_SumIncomingFlowOfSetEqualsSumFlowFromAllNodesToSet_Base(f, S, maxDest - 1); }
+    // intuition: Sum of incomming flow into the first node of the set is equal to flow from all nodes to the first node of the set.
+  }
+
+  lemma Lemma_SumIncomingFlowOfSetEqualsSumFlowFromAllNodesToSet_Step(f: Flow, S: set<Node>, maxSource: nat, maxDest: nat)
+    requires maxSource < V && maxDest < V && maxSource > 0
+    ensures SumIncomingFlowOfSet(f, S, maxSource, maxDest) == SumFlowFromNodeToSet(f, S, maxSource, maxDest) + SumIncomingFlowOfSet(f, S, maxSource - 1, maxDest)
+    decreases maxDest
+  {
+    if maxDest > 0 { Lemma_SumIncomingFlowOfSetEqualsSumFlowFromAllNodesToSet_Step(f, S, maxSource, maxDest - 1); }
+    // intuition: Sum of incomming flow into set from maxSource to maxDestination
+    // is equal to the sum of incoming flow into set from maxSource - 1 to maxDestination + the flow from maxSource to maxDestination.
+  }
+
+  lemma Lemma_SumIncomingFlowOfSetEqualsSumFlowFromAllNodesToSet(f: Flow, S: set<Node>, maxSource: nat, maxDest: nat)
+    requires maxSource < V && maxDest < V
+    ensures SumIncomingFlowOfSet(f, S, maxSource, maxDest) == SumFlowFromAllNodesToSet(f, S, maxSource, maxDest)
+    decreases maxSource
+  {
+    if maxSource == 0 {
+      Lemma_SumIncomingFlowOfSetEqualsSumFlowFromAllNodesToSet_Base(f, S, maxDest);
+    } else {
+      Lemma_SumIncomingFlowOfSetEqualsSumFlowFromAllNodesToSet(f, S, maxSource - 1, maxDest);
+      Lemma_SumIncomingFlowOfSetEqualsSumFlowFromAllNodesToSet_Step(f, S, maxSource, maxDest);
+    }
+  }
+
+  lemma Lemma_NodeInternalFlowCancelsOut(f: Flow, S: set<Node>, v: Node, limit: nat)
+    requires limit < V
+    requires ValidSkewSymmetryConstraint(f)
+    ensures SumFlowFromNodeToSet(f, S, v, limit) + SumFlowFromSetToNode(f, S, v, limit) == 0
+    decreases limit
+  {
+    if limit > 0 { Lemma_NodeInternalFlowCancelsOut(f, S, v, limit - 1); }
+    // intuition: Because of skew symmetry this holds, f[v][w] = -f[w][v]
+  }
+
+  lemma Lemma_InternalFlowStep(f: Flow, S: set<Node>, maxSource: nat, maxDest: nat)
+    requires maxDest < V && maxSource < V
+    requires maxDest > 0 && maxSource < maxDest
+    ensures SumInternalFlowToSet(f, S, maxSource, maxDest) ==
+            SumInternalFlowToSet(f, S, maxSource, maxDest - 1) + (if maxDest in S then SumFlowFromSetToNode(f, S, maxDest, maxSource) else 0)
+    decreases maxSource
+  {
+    if maxSource > 0 { Lemma_InternalFlowStep(f, S, maxSource - 1, maxDest); }
+    // intuition: Sum of internal flow in set limited by maxSource and maxDest
+    // = sum of internal flow in set limited by maxSource and maxDest - 1
+    // + internal flow to maxDest limited by maxSource if maxDest is in the set
+  }
+
+  lemma Lemma_TotalInternalFlowOfSetIsZero(f: Flow, S: set<Node>, limit: nat)
+    requires limit < V
+    requires ValidSkewSymmetryConstraint(f)
+    ensures SumInternalFlowToSet(f, S, limit, limit) == 0
+    decreases limit
+  {
+    if limit > 0 {
+      Lemma_TotalInternalFlowOfSetIsZero(f, S, limit - 1);
+      Lemma_InternalFlowStep(f, S, limit - 1, limit);
+
+      if limit in S { Lemma_NodeInternalFlowCancelsOut(f, S, limit, limit); }
+
+      // Follows from Lemma_InternalFlowStep
+      assert SumInternalFlowToSet(f, S, limit, limit) ==
+            // shown to be 0 by induction
+            SumInternalFlowToSet(f, S, limit - 1, limit - 1)
+            // shown to be 0 by Lemma_NodeInternalFlowCancelsOut
+            + (if limit in S then SumFlowFromSetToNode(f, S, limit, limit) + SumFlowFromNodeToSet(f, S, limit, limit) else 0)
+            // postcondition
+            == 0;
+    }
+  }
+
+  lemma Lemma_SumFlowFromAllNodesEqualsSumInternalFlowPlusSumExternalFlow(f: Flow, S: set<Node>, maxSource: nat, maxDest: nat)
+    requires maxSource < V && maxDest < V
+    ensures SumFlowFromAllNodesToSet(f, S, maxSource, maxDest) == SumInternalFlowToSet(f, S, maxSource, maxDest) + SumExternalFlowToSet(f, S, maxSource, maxDest)
+    decreases maxSource
+  {
+    if maxSource > 0 { Lemma_SumFlowFromAllNodesEqualsSumInternalFlowPlusSumExternalFlow(f, S, maxSource - 1, maxDest); }
+    // intuition: Sum of flow from all nodes to set
+    // equals sum of from from nodes outside of set to set + sum of flow from nodes inside of set to set.
+  }
+
+  lemma Lemma_FlowFromExternalNodeToReachableSetIsNonPositive(c: Capacity, f: Flow, v: Node, S: set<Node>, extNode: Node, limit: nat)
+    requires ValidCapacityConstraint(c, f) && ValidSkewSymmetryConstraint(f)
+    requires S == NodesReachableFrom(c, f, v)
+    requires extNode !in S
+    requires limit < V
+    ensures SumFlowFromNodeToSet(f, S, extNode, limit) <= 0
+    decreases limit
+  {
+    // show postcondition holds for set up to and including limit - 1
+    if limit > 0 { Lemma_FlowFromExternalNodeToReachableSetIsNonPositive(c, f, v, S, extNode, limit - 1); }
+
+    // SumFlowFromNodeToSet only changes if limit is in S
+    if limit in S {
+      // prove residual capacity is 0 by contradiction
+      assert ResidualCapacity(c, f, limit, extNode) == 0 by {
+        if ResidualCapacity(c, f, limit, extNode) > 0 {
+          assert extNode in S by {
+            Lemma_NodeReachableFromReachableSetIsReachable(c, f, v, limit, extNode);
+          }
+          assert false;
+        }
+      }
+
+      assert 0 <= c[limit][extNode] == f[limit][extNode]; // by ValidCapacityConstraint and residual capacity of 0
+      assert f[limit][extNode] == -f[extNode][limit]; // by ValidSkewSymmetryConstraint
+      assert f[extNode][limit] <= 0; // follows from above assertions
+
+      assert SumFlowFromNodeToSet(f, S, extNode, limit) == 
+       (if limit > 0 then SumFlowFromNodeToSet(f, S, extNode, limit - 1) else 0) // <= 0 by induction
+       + (if limit in S then f[extNode][limit] else 0); // <= 0 by inductive step
+    }
+  }
+
+  lemma Lemma_TotalExternalFlowOfReachableSetIsNonPositive(c: Capacity, f: Flow, v: Node, S: set<Node>, maxSource: nat, maxDest: nat)
+    requires ValidCapacityConstraint(c, f) && ValidSkewSymmetryConstraint(f)
+    requires S == NodesReachableFrom(c, f, v)
+    requires maxSource < V && maxDest < V
+    ensures SumExternalFlowToSet(f, S, maxSource, maxDest) <= 0
+    decreases maxSource
+  {
+    // show postcondition holds for set up to and including maxSource - 1
+    if maxSource > 0 { Lemma_TotalExternalFlowOfReachableSetIsNonPositive(c, f, v, S, maxSource - 1, maxDest); }
+    // show that it holds for maxSource
+    if maxSource !in S { Lemma_FlowFromExternalNodeToReachableSetIsNonPositive(c, f, v, S, maxSource, maxDest); }
   }
 }
